platform/AutoSep.v
@@ -7,14 +7,20 @@ Ltac sep hints :=
       match goal with
         | [ |- context[localsInvariant _ _ true _ ?ns'' _ _] ] =>
           let ns' := peelPrefix ns ns'' in
-            intros; eapply (@localsInvariant_in ns'); [
-              eassumption
-              | simpl; omega
-              | reflexivity
-              | reflexivity
-              | repeat constructor; simpl; intuition congruence
-              | intros ? ? Hrew; repeat rewrite Hrew by (simpl; tauto); reflexivity
-              | intros ? ? Hrew; repeat rewrite Hrew by (simpl; tauto); reflexivity ]
+            intros;
+              repeat match goal with
+                       | [ H : interp _ _ |- _ ] =>
+                         eapply localsInvariant_inEx; [ | apply H ];
+                           clear H; simpl; intros
+                     end;
+              eapply (@localsInvariant_in ns'); [
+                eassumption
+                | simpl; omega
+                | reflexivity
+                | reflexivity
+                | repeat constructor; simpl; intuition congruence
+                | intros ? ? Hrew; repeat rewrite Hrew by (simpl; tauto); reflexivity
+                | intros ? ? Hrew; repeat rewrite Hrew by (simpl; tauto); reflexivity ]
       end
     | _ => PreAutoSep.sep hints
   end.
